paired ids

src/HiFirrtl.v
@@ -154,6 +154,10 @@ it does not make sense to put effort in external modules.
 
 End HiFirrtl.
 
+(********************************************************************************)
+
+(** Component Environment *)
+
 Section Component_types.
   (* A mapping from a variable to its component type.
   This mapping is needed because a register or memory definition
@@ -278,6 +282,11 @@ Module MakeCmpntEnv (V : SsrOrder) (VM : SsrFMap with Module SE := V) <:
 End MakeCmpntEnv.
 
 Module CE (*<: CmpntEnv VarOrder *) := MakeCmpntEnv VarOrder VM.
+
+
+(********************************************************************************)
+
+(** Component Connections *)
 
 (* rhs expressions *)
 Section Rhs_expr.
@@ -476,12 +485,121 @@ End MakeStructStore.
 
 Module StructState := MakeStructStore VarOrder CE.
 
+
+
+(********************************************************************************)
+
+(** Identifiers *)
+
+Fixpoint size_of_ftype ft :=
+  match ft with
+  | Gtyp t => 1
+  | Atyp t n => (size_of_ftype t) * n
+  | Btyp b => size_of_fields b
+  end
+with size_of_fields b :=
+       match b with
+       | Fnil => 0
+       | Fflips v fl t fs => (size_of_ftype t) + size_of_fields fs
+       end.
+
+Fixpoint offset_of_subfield_b ft fid n :=
+  match ft with
+  | Fnil => n
+  | Fflips v fl t fs => if fid == v then n else offset_of_subfield_b fs fid (n + size_of_ftype t)
+  end.
+
+Definition offset_of_subfield ft fid n :=
+  match ft with
+  | Gtyp t => 0
+  | Atyp t n => 0
+  | Btyp b => offset_of_subfield_b b fid n
+  end.
+
+Definition offset_of_subindex ft m :=
+  match ft with
+  | Gtyp t => 0
+  | Atyp t n => m
+  | Btyp b => 0
+  end.
+
+(* make modules for paired idents*)
+Module ProdVarOrder := MakeProdOrderWithDefaultSucc VarOrder VarOrder.
+Module PVS <: SsrFSetWithNew := FSets.MakeTreeSetWithNew ProdVarOrder.
+Module PVM <: SsrFMapWithNew := FMaps.MakeTreeMapWithNew ProdVarOrder.
+Module Ids_map2 := Map2 PVS PVS. 
+
+  
+(* idents pair *)
+Definition pvar := ProdVarOrder.t.
+
+
+Section Preprocess.
+  
+  (* index *)
+  Definition initial_index : N := 0.
+  Definition first_index : N := 1.
+  Definition next_index i : N := i + 1.
+
+  (* A map from paired vars to indexes *)
+  Definition ind_map := PVM.t (N * N).
+  Definition ind_map_empty : ind_map := PVM.empty (N * N).
+
+  (* finds in idents_map*)
+  Definition find_base_index (m:ind_map) (v:pvar): option N :=
+    match PVM.find v m with
+    | Some i => Some (fst i)
+    | None => None
+    end.
+
+  Definition find_offset_index (m:ind_map) (v:pvar): option N :=
+    match PVM.find v m with
+    | Some i => Some (snd i)
+    | None => None
+    end.
+
+  Definition acc_indexes (m:ind_map) (v:pvar): N * N :=
+    match PVM.find v m with
+    | Some i => i
+    | None => (initial_index, initial_index)
+    end.
+
+  (* set/get indivual index with base index*)
+  Parameter set_pvar : forall m (p:pvar), acc_indexes m p = p.
+  Definition get_pvar m (p:pvar) : N * N := (p.1%N, N.add (acc_indexes m p).1%N (acc_indexes m p).2%N).
+  
+  Lemma pvar_preserve (m : ind_map) : Ids_map2.preserve (get_pvar m).
+  Proof.
+    move => x y H.
+    rewrite (eqP H) eq_refl//.
+  Qed.
+
+  Lemma pvar_injective (m : ind_map) : Ids_map2.injective (get_pvar m).
+  Proof.
+    move => x y /eqP H. 
+    case : H => H1 H2.
+    move : H2. rewrite !set_pvar.
+    rewrite H1 N.add_cancel_l. move : H1.
+    case x => x1 x2; case y => y1 y2 => /= H1 H2.
+    rewrite H1 H2//.
+  Qed.
+
+  Definition pvar_well m :=
+    Ids_map2.mkWellMap2 (pvar_preserve m) (pvar_injective (m:=m)).
+
+
+  
+End Preprocess.
+
+
 Module MakeHiFirrtl
-       (V : SsrOrder) (* identifier names *)
-       (VS : SsrFSet with Module SE := V)
-       (VM : SsrFMap with Module SE := V)
-       (CE : CmpntEnv V with Module SE := V)
-       (SV : StructStore V CE). (* map from names of defined identifiers to their type and kind *)
+  (V : SsrOrder) (* identifier names *)
+  (PV : SsrOrder) (* identifier names *)
+  (PVS : SsrFSet with Module SE := PV)
+  (VS : SsrFSet with Module SE := V)
+  (VM : SsrFMap with Module SE := V)
+  (CE : CmpntEnv V with Module SE := V)
+  (SV : StructStore V CE). (* map from names of defined identifiers to their type and kind *)
 
   (* Local Open Scope hifirrtl. *)
 
@@ -2591,15 +2709,5 @@ Proof.
 
 End MakeHiFirrtl.
 
-
-Module HiF := MakeHiFirrtl VarOrder VS VM CE StructState.
-
-Section Preprocess.
-
-  Definition initial_index : N := 0.
-
-  Definition first_assigned_index : N := 1.
-
-  Definition 
-  
-End Preprocess.
+(* HiFirrtl module with variables of type N *)
+Module HiF := MakeHiFirrtl VarOrder ProdVarOrder PVS VS VM CE StructState.
